chore: add sorry about logarithmic height

Filrb/Basic.lean
@@ -15,9 +15,9 @@ invariants. Due to Lean's FFI representation this has the same memory layout as 
 -/
 structure Set (α : Type u) [Preorder α] [Ord α] [LawfulOrd α] where
   raw : Internal.Raw α
-  bst: Internal.Raw.BST raw
-  color : Internal.Raw.ChildInv raw
-  height : Internal.Raw.HeightInv raw
+  hbst: Internal.Raw.BST raw
+  hcolor : Internal.Raw.ChildInv raw
+  hheight : Internal.Raw.HeightInv raw
 
 namespace Set
 
@@ -30,9 +30,9 @@ The empty set.
 def empty : Set α :=
   {
     raw := .nil
-    bst := Internal.Raw.bst_nil
-    color := Internal.Raw.childInv_nil
-    height := Internal.Raw.heightInv_nil
+    hbst := Internal.Raw.bst_nil
+    hcolor := Internal.Raw.childInv_nil
+    hheight := Internal.Raw.heightInv_nil
   }
 
 instance : EmptyCollection (Set α) where
@@ -52,9 +52,9 @@ def insert (set : Set α) (x : α) : Set α :=
   let ⟨raw, bst, color, height⟩ := set
   {
     raw := raw.insert x
-    bst := Internal.Raw.bst_insert_of_bst x raw bst
-    color := Internal.Raw.childInv_insert_of_bst x raw color
-    height := Internal.Raw.heightInv_insert_of_bst x raw height
+    hbst := Internal.Raw.bst_insert_of_bst x raw bst
+    hcolor := Internal.Raw.childInv_insert_of_bst x raw color
+    hheight := Internal.Raw.heightInv_insert_of_bst x raw height
   }
 
 /--
@@ -67,7 +67,7 @@ instance : Membership α (Set α) where
   mem set x := x ∈ set.raw
 
 theorem contains_eq_true_iff_mem {set : Set α} {x : α} : set.contains x = true ↔ x ∈ set :=
-  Internal.Raw.contains_eq_true_iff_mem_of_bst set.bst
+  Internal.Raw.contains_eq_true_iff_mem_of_bst set.hbst
 
 instance {x : α} {set : Set α} : Decidable (x ∈ set) :=
   decidable_of_iff (set.contains x) contains_eq_true_iff_mem
@@ -80,9 +80,9 @@ def erase (set : Set α) (x : α) : Set α :=
   let ⟨raw, bst, color, height⟩ := set
   {
     raw := raw.erase x
-    bst := Internal.Raw.bst_erase_of_bst x raw bst
-    color := Internal.Raw.childInv_erase_of_bst x raw color
-    height := Internal.Raw.heightInv_erase_of_bst x raw height
+    hbst := Internal.Raw.bst_erase_of_bst x raw bst
+    hcolor := Internal.Raw.childInv_erase_of_bst x raw color
+    hheight := Internal.Raw.heightInv_erase_of_bst x raw height
   }
 
 /--
@@ -90,6 +90,12 @@ Returns the amount of elements in `set`.
 -/
 @[inline]
 def size (set : Set α) : Nat := set.raw.size
+
+/--
+Returns the height of the tree backing `set`.
+-/
+@[inline]
+def height (set : Set α) : Nat := set.raw.height
 
 end Set
 
